add inconsistency proof and equivalence of transitivity

FormalizingAxiomaticTheoriesOfTruth/TarskisTheorem.lean
@@ -1,6 +1,5 @@
 import FormalizingAxiomaticTheoriesOfTruth.ProofTheory
-import FormalizingAxiomaticTheoriesOfTruth.Syntax
-import FormalizingAxiomaticTheoriesOfTruth.Conservativity
+import FormalizingAxiomaticTheoriesOfTruth.ArithTheories
 open FirstOrder
 open Language
 
@@ -22,7 +21,7 @@ variable {L : Language}
 [DecidableEq (Formula L ℕ)]
 
 def syntax_and_PA : Set (Formula ℒₜ ℕ) :=
-  syntax_theory ∪ peano_arithmetic
+  syntax_theory ∪ 𝐏𝐀𝐓
 
 def unrestricted_TB : Theory ℒₜ :=
   { φ | ∃ ψ : Formula ℒₜ ℕ, φ = (T(⌜ψ⌝) ⇔ ψ) }
@@ -40,7 +39,7 @@ axiom diagonal_lemma
   (φ : BoundedFormula ℒₜ ℕ 0) :
   ∃ (ψ : Formula ℒₜ ℕ),
     syntax_and_PA_unres_TB ⊢
-      (ψ ⇔ (φ/[⌜ψ⌝]))
+      (ψ ⇔ (φ////[⌜ψ⌝]))
 
 -- def bicond_elim (Th: unrestricted_TB) (A B : Formula L ℕ ) :
 --   unrestricted_TB ⊢ A ⇔ B := by
@@ -55,9 +54,109 @@ axiom diagonal_lemma
 --     apply lemma A, B
 
 lemma eqv_trans : ∀Th : Set (Formula L ℕ), ∀(A B C : L.Formula ℕ), Nonempty (Derivation Th {A ⇔ B, C ⇔ B} {A ⇔ C}) := by
+  let eqv_trans_derivation
+    (Th : Set (Formula L ℕ)) (A B C : Formula L ℕ) (h₁ : C = A ∨ C = ∼((A ⟹ B) ⟹ ∼(B ⟹ A)) ∨ C = ∼((C ⟹ B) ⟹ ∼(B ⟹ C))) (h₂ : A = C ∨ A = ∼((A ⟹ B) ⟹ ∼(B ⟹ A)) ∨ A = ∼((C ⟹ B) ⟹ ∼(B ⟹ C))) :
+    Derivation Th {A ⇔ B, C ⇔ B} {A ⇔ C} := by
+    dsimp [FirstOrder.Language.BoundedFormula.iff]
+    dsimp [instMin]
+    apply Derivation.right_conjunction (A ⟹ C) (C ⟹ A) {A ⟹ C} {C ⟹ A} ∅
+    apply Derivation.right_implication A C {A, (A ⟹ B) ⊓ (B ⟹ A), (C ⟹ B) ⊓ (B ⟹ C)} {C} ∅
+    apply Derivation.lax
+    simp
+    dsimp [instMin]
+    exact h₁
+    dsimp [instMin]
+    rw [Finset.insert_eq]
+    rw [Finset.empty_union]
+    rw [Finset.empty_union]
+    rw [Finset.empty_union]
+    apply Derivation.right_implication C A {C, (A ⟹ B) ⊓ (B ⟹ A), (C ⟹ B) ⊓ (B ⟹ C)} {A} ∅
+    apply Derivation.lax
+    simp
+    dsimp [instMin]
+    exact h₂
+    dsimp[instMin]
+    rw [Finset.insert_eq]
+    rw [Finset.empty_union]
+    rw [Finset.empty_union]
+    rw [Finset.empty_union]
+    rw [Finset.empty_union]
+    dsimp [land]
+  intro Th A B C
+  apply eqv_trans_derivation at Th
+  apply Th at A
+  apply A at B
+  apply B at C
+  apply Nonempty.intro
   sorry
 
 lemma inconsistency : ∀Th : Set (Formula L ℕ), ∀(A : L.Formula ℕ), Nonempty (Derivation Th {A ⇔ ∼A} {⊥}) := by
+  let inconsistency_derivation
+    (Th : Set (Formula L ℕ)) (A : Formula L ℕ) (h₁ : ⊥ ∉ {A}) (h₂ : ∼A ∉ {A}) (h₃ : ⊥ ≠ A) (h₄ : A ⟹ ∼A ∈ {A ⟹ ∼A, ∼A ⟹ A}) (h₅ : ∼A ⟹ A ∈ {A ⟹ ∼A, ∼A ⟹ A}) (h₆ : A ⟹ ∼A ≠ ∼A ⟹ A):
+    Derivation Th {A ⇔ ∼A} {⊥} := by
+    dsimp [FirstOrder.Language.BoundedFormula.iff]
+    apply Derivation.left_conjunction (A ⟹ ∼A) (∼A ⟹ A) {(A ⟹ ∼A), (∼A ⟹ A)}
+    apply Derivation.left_implication A ∼A {(∼A ⟹ A)} {⊥, A} {∼A, (∼A ⟹ A)}
+    apply Derivation.left_implication ∼A A ∅ {⊥, A, ∼A} {A}
+    apply Derivation.right_negation A {A} {⊥, A}
+    apply Derivation.lax
+    simp
+    rw [Finset.sdiff_self]
+    rw [Finset.insert_eq]
+    rw [Finset.union_comm]
+    rw [Finset.insert_eq]
+    rw [Finset.insert_eq]
+    rw [Finset.union_comm]
+    rw [Finset.union_assoc]
+    rw [Finset.insert_eq]
+    rw [Finset.insert_eq]
+    rw [Finset.union_comm]
+    rw [Finset.insert_eq]
+    rw [Finset.union_comm]
+    rw [Finset.union_assoc]
+    apply Derivation.lax
+    simp
+    rw [Finset.union_empty]
+    rw [Finset.empty_union]
+    rw [Finset.insert_eq]
+    apply Derivation.left_implication ∼A A {∼A} {⊥, ∼A} {A, ∼A}
+    apply Derivation.right_negation A {∼A, A} {⊥}
+    apply Derivation.left_negation A {A} {⊥, A}
+    apply Derivation.lax
+    simp
+    rw [Finset.insert_eq]
+    rw [Finset.union_comm]
+    rw [Finset.insert_sdiff_cancel]
+    exact h₁
+    rw [Finset.insert_sdiff_cancel]
+    exact h₂
+    rw [Finset.insert_eq]
+    rw [Finset.insert_eq]
+    apply Derivation.left_negation A {A} {⊥, A}
+    apply Derivation.lax
+    simp
+    rw [Finset.insert_eq]
+    rw [Finset.insert_sdiff_cancel]
+    rw [Finset.not_mem_singleton]
+    exact h₃
+    rw [Finset.insert_eq]
+    rw [Finset.insert_eq]
+    rw [Finset.insert_eq]
+    rw [Finset.insert_eq]
+    rw [Finset.union_comm]
+    exact h₄
+    exact h₅
+    rw [Finset.insert_eq]
+    rw [Finset.union_sdiff_cancel_left]
+    rw [Finset.sdiff_self]
+    rw [Finset.empty_union]
+    dsimp [land, instMin]
+    rw [Finset.disjoint_singleton]
+    exact h₆
+  intro Th A
+  apply inconsistency_derivation at Th
+  apply Th at A
+  apply Nonempty.intro
   sorry
 
 def false_formula : Formula ℒₜ ℕ := ⊥
@@ -71,23 +170,22 @@ theorem tarskis_theorem : syntax_and_PA_unres_TB ⊢ false_formula := by
   -- --     -- apply diagonal_lemma φ
   -- --     -- sorry
       let φ : BoundedFormula ℒₜ ℕ 0 := ∼T(var (Sum.inl 0))
-      have step1 : {t : ℒₜ.Term (ℕ ⊕ Fin 0)} → φ////[t] = ∼T(t)
-        | .var v => match v with
+      -- have step1 : {t : ℒₜ.Term (ℕ ⊕ Fin 0)} → φ////[t] = ∼T(t)
+      --   | .var v => match v with
+      --   | _ => sorry
 
-        | _ => sorry
+      -- have step2 {ψ : Formula ℒₜ ℕ} : (φ////[⌜ψ⌝]) = ∼T(⌜ψ⌝) := by
+      --   simp[φ, my_subst]
+      --   sorry
 
-      have step2 {ψ : Formula ℒₜ ℕ} : (φ/[⌜ψ⌝]) = ∼T(⌜ψ⌝) := by
-        simp[φ,my_subst]
-
-      apply diagonal_lemma φ
-  --     apply diagonal_lemma φ
-
+      -- apply diagonal_lemma φ
   --     -- use ψ
   --     -- rw [th_to_set_form]
   -- -- rw [this] at hψ
   -- -- use ψ
   -- -- exact hψ
-  obtain ⟨ψ, liar_formula_der⟩ := liar_formula_exists
+      sorry
+  obtain ⟨ψ⟩ := liar_formula_exists
   -- have liar_formula_exists :
   --   ∃ (ψ : Formula ℒₜ ℕ),
   --     syntax_and_PA_unres_TB ⊢ (ψ ⇔ (∼T(var (Sum.inl 0)))////[⌜ψ⌝]) := by
@@ -96,14 +194,16 @@ theorem tarskis_theorem : syntax_and_PA_unres_TB ⊢ false_formula := by
   have liar_t_instance : syntax_and_PA_unres_TB ⊢ (T(⌜ψ⌝) ⇔ ψ) := by
     sorry
   -- Step 3: Derive T(⌜ψ⌝) ⇔ ∼T(⌜ψ⌝)
-  have intermediate_lemma :
-    syntax_and_PA_unres_TB ⊢ (T(⌜ψ⌝) ⇔ ∼T(⌜ψ⌝)) := by
+  have intermediate_lemma : syntax_and_PA_unres_TB ⊢ (T(⌜ψ⌝) ⇔ ∼T(⌜ψ⌝)) := by
       obtain ⟨derivation⟩ := eqv_trans syntax_and_PA_unres_TB (T(⌜ψ⌝)) (∼T(⌜ψ⌝)) ψ
       sorry
   obtain ⟨d⟩ := inconsistency (th_to_set_form syntax_and_PA_unres_TB) (T(⌜ψ⌝))
   sorry
 
 
+  lemma test {t t' : ℒ.Term (ℕ ⊕ Fin 0)} : ((var (Sum.inl 0) =' t)////[t']) = (t' =' t):= by
+    #check ((var (Sum.inl 0) =' t)////[t'])
+    #check t' =' t
 
 
 
